chore: rename `insert_emptyc_eq` to `insert_empty_eq` (#7451)
This PR renames the member `insert_emptyc_eq` of the `LawfulSingleton`
typeclass to `insert_empty_eq` to conform to the recommended spelling of
`∅` as `empty`.

See also #7447.

src/Init/Core.lean
@@ -514,10 +514,21 @@ export Singleton (singleton)
 class LawfulSingleton (α : Type u) (β : Type v) [EmptyCollection β] [Insert α β] [Singleton α β] :
     Prop where
   /-- `insert x ∅ = {x}` -/
-  insert_emptyc_eq (x : α) : (insert x ∅ : β) = singleton x
-export LawfulSingleton (insert_emptyc_eq)
+  insert_empty_eq (x : α) : (insert x ∅ : β) = singleton x
+export LawfulSingleton (insert_empty_eq)
 
-attribute [simp] insert_emptyc_eq
+attribute [simp] insert_empty_eq
+
+@[deprecated insert_empty_eq (since := "2025-03-12")]
+theorem insert_emptyc_eq [EmptyCollection β] [Insert α β] [Singleton α β]
+    [LawfulSingleton α β] (x : α) : (insert x ∅ : β) = singleton x :=
+  insert_empty_eq _
+
+@[deprecated insert_empty_eq (since := "2025-03-12")]
+theorem LawfulSingleton.insert_emptyc_eq [EmptyCollection β] [Insert α β] [Singleton α β]
+    [LawfulSingleton α β] (x : α) : (insert x ∅ : β) = singleton x :=
+  insert_empty_eq _
+
 
 /-- Type class used to implement the notation `{ a ∈ c | p a }` -/
 class Sep (α : outParam <| Type u) (γ : Type v) where
